WIP: Triples for SL

backends/lean/Aeneas/Std/WP.lean
@@ -1,69 +1,110 @@
 import Aeneas.Std.Primitives
 import Std.Do
+import Iris.BI
+import Iris.Std.Heap
+-- import Iris.ProofMode
+import Nola
 
 namespace Aeneas.Std.WP
 
+axiom GF : Iris.BundledGFunctors
+abbrev sProp := aProp.{1} GF -- TODO: we have to be constant in the universe,
+                             -- otherwise we have problems when lifting from Pure
+
+-- open Iris.BI
 open Std
 
-def Post α := (α -> Prop)
-def Pre := Prop
 
-def Wp α := Post α → Pre
+abbrev Post α := (α -> Prop)
+abbrev Pre := Prop
+abbrev SLPost (α:Type) := (α → sProp)
+abbrev SLPre := sProp
 
-def wp_return (x:α) : Wp α := fun p => p x
 
+theorem proof_example_1 (P Q R : sProp) (Φ : SLPost α) :
+  P ∗ Q ∗ □ R ⊢ □ (R -∗ ∃ x, Φ x) -∗ ∃ x, Φ x ∗ P ∗ Q
+:= by
+  iintro ⟨HP, HQ, □HR⟩ □HRΦ
+  ispecialize HRΦ HR as HΦ
+  icases HΦ with ⟨x, _HΦ⟩
+  iexists x
+  isplitr
+  · iassumption
+  isplitl [HP]
+  · iexact HP
+  · iexact HQ
+
+def Wp (α : Type) := SLPost α → SLPre
+def wp_return (x:α) : Wp α :=
+  fun p => p x
 def wp_bind (m:Wp α) (k:α -> Wp β) : Wp β :=
   fun p => m (fun r => k r p)
 
-def wp_ord (wp1 wp2:Wp α) :=
-  forall p, wp1 p → wp2 p
-
+noncomputable
 def theta (m:Result α) : Wp α :=
   match m with
   | .ok x => wp_return x
-  | .fail _ => fun _ => False
-  | .div => fun _ => False
+  | .fail _ => fun _ => iprop(⌜False⌝)
+  | .div => fun _ => iprop(⌜False⌝)
 
-def p2wp (post:Post α) : Wp α :=
-  fun p => forall r, post r → p r
+-- def p2wp (post:Post α) : Wp α :=
+--   fun p => forall r, post r → p r
 
-def spec_general (x:Result α) (p:Post α) :=
-  wp_ord (p2wp p) (theta x)
+-- def spec_general (x:Result α) (p:Post α) :=
+--   wp_ord (p2wp p) (theta x)
 
-def spec (x:Result α) (p:Post α) :=
-  theta x p
+noncomputable
+def lift_to_SLPost (Q:Post α) : SLPost α :=
+  fun v => iprop(⌜Q v⌝)
 
+def slspec (P:SLPre) (x:Result α) (Q:SLPost α) :=
+  P ⊢ theta x Q
+
+def spec (x:Result α) (Q:Post α) :=
+  slspec iprop(True) x (lift_to_SLPost Q)
+
+-- Proofs about spec
 @[simp, grind =]
-theorem spec_ok (x : α) : spec (.ok x) p ↔ p x := by simp [spec, theta, wp_return]
+theorem spec_ok (x : α) : spec (.ok x) Q ↔ Q x := by
+  simp [spec, slspec, lift_to_SLPost, theta, wp_return]
+  apply Iff.intro
+  · intro h
+    sorry -- Cezar: I think it duable
+  · intro h
+    ipure_intro
+    intro
+    exact h
 
-theorem spec_bind {k:α -> Result β} {Pₖ:Post β} {m:Result α} {Pₘ:Post α} :
-  spec m Pₘ →
-  (forall x, Pₘ x → spec (k x) Pₖ) →
-  spec (Std.bind m k) Pₖ := by
+theorem spec_ok_l (x : α) : spec (.ok x) Q → Q x := by
+  sorry
+
+theorem spec_bind {k:α -> Result β} {Qₖ:Post β} {m:Result α} {Qₘ:Post α} :
+  spec m Qₘ →
+  (forall x, Qₘ x → spec (k x) Qₖ) →
+  spec (Std.bind m k) Qₖ := by
   intro Hm Hk
   cases m
   · simp
     apply Hk
-    apply Hm
+    apply (spec_ok_l _ Hm)
   · simp
     apply Hm
   · simp
     apply Hm
 
-theorem spec_mono {P₁:Post α} {m:Result α} {P₀:Post α} (h : spec m P₀):
-  (∀ x, P₀ x → P₁ x) → spec m P₁ := by
+theorem spec_mono {Q₁:Post α} {m:Result α} {Q₀:Post α} (h : spec m Q₀):
+  (∀ x, Q₀ x → Q₁ x) → spec m Q₁ := by
   intros HMonPost
   revert h
-  unfold spec theta wp_return
-  cases m <;> grind
+  sorry
 
 theorem progress_spec_equiv_exists (m:Result α) (P:Post α) :
   spec m P ↔ (∃ y, m = .ok y ∧ P y) :=
   by
     cases m
-    · simp [spec, theta, wp_return]
-    · simp [spec, theta]
-    · simp [spec, theta]
+    · sorry
+    · sorry
+    · sorry
 
 theorem progress_spec_exists {m:Result α} {P:Post α} :
   spec m P → (∃ y, m = .ok y ∧ P y) := by
@@ -73,15 +114,64 @@ theorem progress_exists_spec {m:Result α} {P:Post α} :
   (∃ y, m = .ok y ∧ P y) → spec m P := by
   exact (progress_spec_equiv_exists m P).2
 
-scoped syntax:lead (name := specSyntax) term:lead " ⦃" "⇓" term " => " term "⦄" : term
+
+-- Proofs about slspec
+theorem slspec_ok (P:SLPre) (x : α) (Q:SLPost α): slspec P (.ok x) Q ↔ P ⊢ Q x := by
+  simp [slspec, theta, wp_return]
+
+theorem slspec_frame (m:Result α) :
+  slspec P m Q →
+  (forall F, slspec iprop(P ∗ F) m (fun x => iprop(Q x ∗ F))) := by
+  intro Hspec F
+  sorry
+
+theorem slspec_mono
+  {P₁:SLPre} {Q₁:SLPost α} {m:Result α}
+  (P₀:SLPre) (Q₀:SLPost α) (h : slspec P₀ m Q₀) :
+  (⊢ P₁ -∗ P₀) →
+  (∀ x, Q₀ x ⊢ Q₁ x) →
+  slspec P₁ m Q₁ := by
+  intros HMonPre HMonPost
+  sorry
+
+theorem slspec_bind {k:α -> Result β} {P:SLPre} {Qₖ:SLPost β} {m:Result α} {Pₘ:SLPre} {Qₘ:SLPost α} :
+  slspec Pₘ m Qₘ →
+  (⊢ P -∗ Pₘ ∗ F) →
+  (forall x, slspec iprop((Qₘ x) ∗ F) (k x) Qₖ) →
+  slspec P (Std.bind m k) Qₖ := by
+  intro Hm Hk Hx
+  cases m
+  · rename_i x
+    simp
+    apply slspec_mono iprop((Qₘ x) ∗ F) Qₖ
+    · apply Hx
+    · sorry
+    · sorry
+    -- · have := slspec_frame (.ok x) Hm F
+    -- apply (slspec_ok _ _ Hm)
+  · sorry
+  · sorry
+
+scoped syntax:lead (name := specSyntax) "(" term:lead ")" " ⦃" "⇓ " Lean.Parser.Term.funBinder " => " term " ⦄" : term
+scoped syntax:lead (name := specSyntaxPred) "(" term:lead ")" " ⦃" "⇓ " term " ⦄" : term
+scoped syntax:lead (name := slSpecSyntax) " ⦃" term " ⦄" term:lead " ⦃" "⇓ " Lean.Parser.Term.funBinder " => " term " ⦄" : term
+scoped syntax:lead (name := slSpecSyntaxPred) " ⦃" term " ⦄" term:lead " ⦃" "⇓ " term " ⦄" : term
 
 macro_rules
-  | `($x ⦃⇓ $r => $P⦄)  => `(Aeneas.Std.WP.spec $x (fun $r => $P))
+  | `(($x) ⦃⇓ $r => $Q⦄)  => `(Aeneas.Std.WP.spec $x (fun $r => $Q))
+  | `(($x) ⦃⇓ $Q:term⦄)  => `(Aeneas.Std.WP.spec $x $Q)
+  | `(⦃$P⦄ $x ⦃⇓ $r =>  $Q⦄)  => `(Aeneas.Std.WP.slspec $x $P (fun $r => $Q))
+  | `(⦃$P⦄ $x ⦃⇓ $Q⦄)  => `(Aeneas.Std.WP.slspec $x $P $Q)
+-- scoped syntax:lead (name := slspecSyntax)
+--   " ⦃" term "⦄" term:lead " ⦃" "⇓" term " => " term "⦄" : term
 
-example : .ok 0 ⦃⇓ r => r = 0⦄ := by simp
+-- macro_rules
+--   | `(⦃$P⦄ $x ⦃⇓ $r => $Q⦄)  => `(Aeneas.Std.WP.slspec $P $x (fun $r => $Q))
+
+example : (.ok 0) ⦃⇓ r => r = 0⦄ := by simp
 
 def add1 (x : Nat) := Result.ok (x + 1)
-theorem  add1_spec (x : Nat) : add1 x ⦃⇓ y => y = x + 1⦄ :=
+theorem  add1_spec (x : Nat) : (add1 x) ⦃⇓ y => y = x + 1⦄ :=
   by simp [add1]
 
 example (x : Nat) :
@@ -98,7 +188,7 @@ example (x : Nat) :
     grind
 
 def add2 (x : Nat) := Result.ok (x + 1, x + 2)
-theorem  add2_spec (x : Nat) : add2 x ⦃⇓ (y, z) => y = x + 1 ∧ z = x + 2⦄ :=
+theorem  add2_spec (x : Nat) : (add2 x) ⦃⇓ (y, z) => y = x + 1 ∧ z = x + 2⦄ :=
   by simp [add2]
 
 example (x : Nat) :
@@ -121,6 +211,34 @@ example (x : Nat) :
     clear tmp
     --
     grind
+
+-- TODO:
+-- noncomputable
+-- example incr_ptr (p : RawPtr U32) : ITree Unit := do
+--   let x0 ← read_ptr p
+--   let x1 ← UScalar.add x0 1#u32
+--   write_ptr p x1
+
+-- def RawPtr (_ : Type) := Nat
+-- axiom ptr {α} : RawPtr α → α → HProp
+
+-- macro:max x:term " ~> " y:term : term => `(ptr $x $y)
+
+-- axiom mut_to_raw {α} (x : α) : Result (RawPtr α)
+-- axiom mut_to_raw.spec {α} (x : α) : ⦃ ∅ ⦄ (mut_to_raw x) ⦃ fun p => p ~> x ⦄
+-- axiom end_mut_to_raw {α} (p : RawPtr α) : Result α
+-- axiom end_mut_to_raw.spec {α : Type} {x : α} (p : RawPtr α) :
+--   ⦃ p ~> x ⦄ (end_mut_to_raw p) ⦃ fun _ => ∅ ⦄
+
+
+-- axiom read_ptr {α : Type} (p : RawPtr α) : ITree α
+-- axiom write_ptr {α : Type} (p : RawPtr α) (x : α) : ITree Unit
+
+-- axiom read_ptr.spec {α} {x : α} {p : RawPtr α} :
+--   ⦃ p ~> x ⦄ (read_ptr p) ⦃ fun _ => p ~> x ⦄ {{ fun x' => x' = x }}
+
+-- axiom write_ptr.spec {α} {x x' : α} {p : RawPtr α} :
+--   ⦃ p ~> x ⦄ (write_ptr p x') ⦃ fun _ => p ~> x' ⦄ {{ fun () => True }}
 
 
 end Aeneas.Std.WP
